Locally_Nameless_Lambda_Calculus/LN_HO_Typing.thy
@@ -1,32 +1,50 @@
 theory LN_HO_Typing
-  imports LN_HO_Term
+  imports
+    LN_HO_Term
 begin
 
-datatype 'ty ty = Base 'ty | Fun "'ty ty" "'ty ty"
-                               
-inductive has_type :: "('f \<rightharpoonup> 'ty ty) \<Rightarrow> ('v \<rightharpoonup> 'ty ty) \<Rightarrow> ('f, 'v) term \<Rightarrow> 'ty ty \<Rightarrow> bool"
+datatype ('\<alpha>, '\<kappa>) ty =
+  TyVar '\<alpha> |
+  TyCtr '\<kappa> "('\<alpha>, '\<kappa>) ty list" |
+  TyBool |
+  TyFun "('\<alpha>, '\<kappa>) ty" "('\<alpha>, '\<kappa>) ty"
+
+type_synonym ('\<alpha>, '\<kappa>) const_ty = "'\<alpha> list \<times> ('\<alpha>, '\<kappa>) ty list \<times> ('\<alpha>, '\<kappa>) ty"
+
+inductive has_type ::
+  "('c \<rightharpoonup> ('\<alpha>, '\<kappa>) const_ty) \<Rightarrow> ('f \<rightharpoonup> ('\<alpha>, '\<kappa>) ty) \<Rightarrow>
+    (('\<alpha>, '\<kappa>) ty, 'c, 'f) preterm \<Rightarrow> ('\<alpha>, '\<kappa>) ty \<Rightarrow> bool"
   for \<C> where
-  Const: "has_type \<C> \<F> (Const c) \<tau>"
-    if "\<C> c = Some \<tau>"
-    for \<F> c \<tau> |
+  Const: "has_type \<C> \<F> (Const c \<tau>\<^sub>1s ts) \<tau>\<^sub>3"
+    if "\<C> c = Some (\<alpha>s, \<tau>\<^sub>2s, \<tau>\<^sub>3)" and "length \<tau>\<^sub>1s = length \<alpha>s" and "list_all2 (has_type \<C> \<F>) ts \<tau>\<^sub>2s"
+    for \<F> c \<tau>\<^sub>1s ts \<tau>\<^sub>3 |
   Free: "has_type \<C> \<F> (Free f) \<tau>"
     if "\<F> f = Some \<tau>"
     for \<F> f \<tau> |
   App: "has_type \<C> \<F> (App t\<^sub>1 t\<^sub>2) \<tau>\<^sub>2"
     if "has_type \<C> \<F> t\<^sub>1 (Fun \<tau>\<^sub>1 \<tau>\<^sub>2)" and "has_type \<C> \<F> t\<^sub>2 \<tau>\<^sub>1"
     for \<F> t\<^sub>1 t\<^sub>2 \<tau>\<^sub>1 \<tau>\<^sub>2 |
-  Abs: "has_type \<C> \<F> (Abs t) (Fun \<tau>\<^sub>1 \<tau>\<^sub>2)"
+  Abs: "has_type \<C> \<F> (Abs \<tau>\<^sub>1 t) (TyFun \<tau>\<^sub>1 \<tau>\<^sub>2)"
     if "\<And>x. x |\<notin>| \<X> \<Longrightarrow> has_type \<C> (\<F>(x \<mapsto> \<tau>\<^sub>1)) (subst_bound 0 (Free x) t) \<tau>\<^sub>2"
     for \<F> t \<tau>\<^sub>1 \<tau>\<^sub>2 \<X>
 
 lemma locally_closed_if_has_type[intro]: "has_type \<C> \<F> t \<tau> \<Longrightarrow> locally_closed t"
-  by (induction \<F> t \<tau> rule: has_type.induct) (auto intro: locally_closed.intros)
+proof (induction \<F> t \<tau> rule: has_type.induct)
+  case (Const \<F> c \<tau>\<^sub>1s ts \<tau>\<^sub>3 \<alpha>s \<tau>\<^sub>2s)
+  show ?case
+  proof (rule locally_closed.Const)
+    show "list_all locally_closed ts"
+      using Const.IH
+      by (simp add: list_all2_conv_all_nth list_all_length)
+  qed
+qed (auto intro: locally_closed.intros)
+
 
 lemma has_type_weaken_funenv: "has_type \<C> \<F> t \<tau>\<^sub>1 \<Longrightarrow> x \<notin> dom \<F> \<Longrightarrow> has_type \<C> (\<F>(x \<mapsto> \<tau>\<^sub>2)) t \<tau>\<^sub>1"
 proof (induction \<F> t \<tau>\<^sub>1 rule: has_type.induct)
-  case (Const \<F> c \<tau>)
+  case (Const \<F> c \<tau>\<^sub>1s ts \<tau>\<^sub>3 \<alpha>s \<tau>\<^sub>2s)
   then show ?case
-    by (auto intro: has_type.intros)
+    by (simp add: has_type.Const list_all2_mono)
 next
   case (Free \<F> f \<tau>)
   then show ?case
@@ -44,16 +62,21 @@ next
     show "has_type \<C> (\<F>(x \<mapsto> \<tau>\<^sub>2, y \<mapsto> \<tau>\<^sub>1)) (subst_bound 0 (Free y) t) \<tau>\<^sub>3"
     proof (cases "x = y")
       case True
+
       then have "\<F>(x \<mapsto> \<tau>\<^sub>2, y \<mapsto> \<tau>\<^sub>1) = \<F>(y \<mapsto> \<tau>\<^sub>1)"
         by simp
+
       then show ?thesis
         using Abs.hyps \<open>y |\<notin>| \<X>\<close> by metis
     next
       case False
+
       then have "\<F>(x \<mapsto> \<tau>\<^sub>2, y \<mapsto> \<tau>\<^sub>1) = \<F>(y \<mapsto> \<tau>\<^sub>1, x \<mapsto> \<tau>\<^sub>2)"
         by auto
+
       moreover have "x \<notin> dom (\<F>(y \<mapsto> \<tau>\<^sub>1))"
         using \<open>x \<notin> dom \<F>\<close> \<open>x \<noteq> y\<close> by simp
+
       ultimately show ?thesis
         using Abs.IH \<open>y |\<notin>| \<X>\<close> by metis
     qed
@@ -61,15 +84,15 @@ next
 qed
 
 lemma has_type_subst_free:
-  fixes t :: "('f, 'v) term"
-  assumes inf_vars: "infinite (UNIV :: 'v set)"
+  fixes t :: "(('\<alpha>, '\<kappa>) ty, 'c, 'f) preterm"
+  assumes inf_vars: "infinite (UNIV :: 'f set)"
   assumes "has_type \<C> \<F> t \<tau>\<^sub>1" and "finite (dom \<F>)" and "\<F> x = Some \<tau>\<^sub>2" and "has_type \<C> \<F> u \<tau>\<^sub>2"
   shows "has_type \<C> \<F> (subst_free x u t) \<tau>\<^sub>1"
   using assms(2-5)
 proof (induction \<F> t \<tau>\<^sub>1 rule: has_type.induct)
-  case (Const \<F> c \<tau>)
+  case (Const \<F> c \<tau>\<^sub>1s ts \<tau>\<^sub>3 \<alpha>s \<tau>\<^sub>2s)
   then show ?case
-    by (auto intro: has_type.intros)
+    by (simp add: has_type.Const list_all2_mono)
 next
   case (Free \<F> f \<tau>)
   then show ?case
